

# Econ 702 Game Theory Problem Set 1 Solution

Weikai Chen

February 5, 2020

**Exercise 2.** Prove that completeness implies reflexivity.

*Proof.* For all  $x \in X$ , either  $x \succeq x$  or  $x \preceq x$  by completeness. Then  $x \succeq x$ .  $\square$

**Exercise 4.**

1. Prove that if there exists a utility function  $u$  that represents  $\succeq$ , then  $\succeq$  is complete and transitive.
2. Does this part of the theorem depend on the assumption that  $X$  is finite?

*Solution.*

1. By the completeness of  $\geq$  on  $\mathbb{R}$ , for any  $x, y \in X$ , we have either

$$u(x) \geq u(y) \text{ or } u(y) \geq u(x)$$

then either  $x \succeq y$  or  $y \succeq x$ , since  $u$  represents  $\succeq$ . Thus, the  $\succeq$  is complete.

Suppose  $x \succeq y$  and  $y \succeq z$ , then we have  $u(x) \geq u(y)$  and  $u(y) \geq u(z)$ . Therefore, by the transitivity of  $\geq$  on  $\mathbb{R}$  we have  $u(x) \geq u(z)$  and then  $x \succeq z$ . Thus,  $\succeq$  is transitive.

2. No.

$\square$

**Exercise 8.** Prove that if  $\preceq$  has a representation of the expected utility form, then  $\preceq$  satisfies the four axioms.

*Proof.* Suppose that  $\preceq$  has a representation of the expected utility form  $U(l) = U(p_1, \dots, p_n) = \sum_k p_k u_k$ . Then

$$U(\alpha l + (1 - \alpha)l'') = \sum_k [\alpha p_k + (1 - \alpha)p_k''] u_k = \alpha U(l) + (1 - \alpha)U(l'') \quad (1)$$

**Continuity.** If  $l \prec l' \prec l''$ , let  $U(l) = a, U(l') = b, U(l'') = c$ , then  $a < b < c$ .  
Let

$$\alpha = \frac{c - b}{c - a}$$

then  $\alpha \in (0, 1)$  and

$$\begin{aligned} U(\alpha l + (1 - \alpha)l'') &= \alpha U(l) + (1 - \alpha)U(l'') \\ &= \frac{c - b}{c - a}a + \frac{c - b}{c - a}c \\ &= \frac{cb - ac + ac - ba}{c - a} \\ &= b = U(l') \end{aligned}$$

Therefore,  $\alpha l + (1 - \alpha)l'' \sim l'$ .

**Independence.** For all  $l, l', l''$  and all  $\alpha \in (0, 1)$ , by (1) we have

$$\begin{aligned} l \preceq l' &\Leftrightarrow U(l) \leq U(l') \\ &\Leftrightarrow \alpha U(l) + (1 - \alpha)U(l'') \leq \alpha U(l') + (1 - \alpha)U(l'') \\ &\Leftrightarrow U(\alpha l + (1 - \alpha)l'') \leq U(\alpha l' + (1 - \alpha)l'') \\ &\Leftrightarrow \alpha l + (1 - \alpha)l'' \preceq \alpha l' + (1 - \alpha)l'' \end{aligned}$$

For completeness and transitivity, see the proof in **Exercise 4**.  $\square$

**Exercise 9.** Show that for all lotteries  $l$  in  $\Delta$ ,  $\delta_1 \preceq l \preceq \delta_n$  when  $n > 3$ .

*Proof.* Note that  $\delta_1 = p_1\delta_1 + p_2\delta_1 + \cdots + p_n\delta_1$ ,  $\delta_n = p_1\delta_n + \cdots + p_n\delta_n$  and

$$l = (p_1, \dots, p_n) = p_1\delta_1 + p_2\delta_2 + \cdots + p_n\delta_n$$

Then by independence and transitivity we have  $\delta_1 \preceq l \preceq \delta_n$  when  $n = 2$ . Suppose that it holds when  $n = k - 1$ , then for  $n = k$ , we have

$$\begin{aligned} \delta_1 &= (p_1\delta_1 + p_2\delta_1 + \cdots + p_{k-2}\delta_1 + p_{k-1}\delta_1) + p_k\delta_1 \\ &\preceq (1 - p_k) \frac{1}{1 - p_k} (p_1\delta_1 + p_2\delta_1 + \cdots + p_{k-2}\delta_1 + p_{k-1}\delta_1) + p_k\delta_k \text{ (independence)} \\ &\preceq (1 - p_k)l + p_k\delta_k = l \text{ (induction hypothesis)} \\ &\preceq p_1\delta_k + (p_2\delta_2 + \cdots + p_{k-1}\delta_{k-1} + p_k\delta_k) \\ &\preceq p_1\delta_k + (1 - p_1)\delta_k = \delta_k \end{aligned}$$

$\square$

**Exercise 10.** Suppose that we have

$$f(\alpha l + (1 - \alpha)l') = \alpha f(l) + (1 - \alpha)f(l')$$

Use the above lemma to derive the following lemma when  $n > 3$ : for any  $l = (p_1, \dots, p_n)$ ,  $f(l) = \sum_k p_k u_k$  where  $u_k = f(\delta_k)$ .

*Proof.* Let  $K = \min\{k : \sum_{i=1}^k p_i = 1\}$  then for any  $k \leq K$  we have  $\sum_{i=k}^n p_i = 1 - \sum_{i=1}^{k-1} p_i > 0$  and  $p_k = 0$  for all  $k > K$ . Then

$$l = p_1\delta_1 + \cdots + p_K\delta_K$$

and

$$\begin{aligned}
f(l) &= f(p_1\delta_1 + (1-p_1)\sum_{i=2}^K \frac{p_i}{1-p_1}\delta_i) = p_1f(\delta_1) + (1-p_1)f(\sum_{i=2}^K \frac{p_i}{1-p_1}\delta_i) \\
&= p_1u_1 + (1-p_1)f(\frac{p_2}{1-p_1}\delta_2 + \frac{1-p_1-p_2}{1-p_1}\sum_{i=3}^K \frac{p_i}{1-p_1-p_2}\delta_i) \\
&= p_1u_1 + p_2u_2 + (1-p_1-p_2)f(\sum_{i=3}^K \frac{p_i}{1-p_1-p_2}\delta_i) \\
&\dots \\
&= p_1u_1 + \dots + p_{K-1}u_{K-1} + (1-p_1-\dots-p_{K-1})f(\frac{p_K}{1-p_1-\dots-p_{K-1}}\delta_K) \\
&= \sum_{k=1}^K p_k u_k = \sum_{k=1}^n p_k u_k
\end{aligned}$$

□

**Exercise 11.** Prove the following **Theorem**  $u = (u_1, \dots, u_n)$  and  $v = (v_1, \dots, v_n)$  represent the same vNM preference relation if and only if there exist numbers  $a > 0$  and  $b$  such that for all  $k$ ,  $v_k = au_k + b$ .

*Proof.* ( $\Leftarrow$ ) For any  $l = (p_1, \dots, p_n) \in \Delta$  we have

$$v(l) = \sum_k p_k v_k = \sum_k p_k (au_k + b) = a \sum_k p_k u_k + nb = au(l) + nb$$

Then for any  $l, l' \in \Delta$ ,

$$u(l) \geq u(l') \Leftrightarrow au(l) + nb \geq au(l') + nb \Leftrightarrow v(l) \geq v(l')$$

( $\Rightarrow$ ) Without loss of generality, assume that  $\delta_1 \preceq \delta_2 \preceq \dots \preceq \delta_n$  and  $\delta_1 \prec \delta_n$ . By continuity, for all  $i$ , there exist  $\alpha_i \in [0, 1]$  such that  $\delta_i \sim \alpha_i \delta_1 + (1 - \alpha_i) \delta_n$ . Since  $u$  and  $v$  represent the  $\preceq$ , for all  $i$

$$\begin{aligned}
u_i &= \alpha_i u_1 + (1 - \alpha_i) u_n = u_n - \alpha_i (u_n - u_1) \\
v_i &= \alpha_i v_1 + (1 - \alpha_i) v_n = v_n - \alpha_i (v_n - v_1)
\end{aligned}$$

Then

$$v_i = v_n - \frac{v_n - v_1}{u_n - u_1} (u_n - u_i)$$

Let

$$\begin{aligned}
a &= \frac{v_n - v_1}{u_n - u_1} > 0 \\
b &= v_n - au_n
\end{aligned}$$

then we have  $v_i = au_i + b, \forall i$

□

**Exercise 12.** Prove the following Proposition.

1. An agent is risk neutral if for all  $x, y \in \mathbb{R}$  and all  $\lambda \in [0, 1]$ ,  $\lambda u(x) + (1 - \lambda)u(y) = u(\lambda x + (1 - \lambda)y)$
2. An agent is risk averse if for all  $x, y \in \mathbb{R}$  and all  $\lambda \in [0, 1]$ ,  $\lambda u(x) + (1 - \lambda)u(y) \leq u(\lambda x + (1 - \lambda)y)$
3. An agent is risk loving if for all  $x, y \in \mathbb{R}$  and all  $\lambda \in [0, 1]$ ,  $\lambda u(x) + (1 - \lambda)u(y) \geq u(\lambda x + (1 - \lambda)y)$

*Proof.* I prove the case of risk averse by induction. For any lottery  $L = (p_1, x_1; \dots, p_n, x_n)$ , it is sufficient to show that

$$U(L) = \sum_{i=1}^n p_i u(x_i) \leq u\left(\sum_{i=1}^n p_i x_i\right) = u(\delta_{\mu_L})$$

by the concavity of  $u$ . It holds when  $n = 2$ . Suppose that it holds for  $n = k - 1$ . When  $n = k$ , for some  $p_j \neq 1$ ,

$$\begin{aligned} u\left(\sum_{i=1}^k p_i x_i\right) &= u\left(p_j x_j + (1 - p_j) \sum_{i \neq j} \frac{p_i}{1 - p_j} x_i\right) \\ &\geq p_j u(x_j) + (1 - p_j) u\left(\sum_{i \neq j} \frac{p_i}{1 - p_j} x_i\right) \text{ by concavity of } u \\ &\geq p_j u(x_j) + (1 - p_j) \sum_{i \neq j} \frac{p_i}{1 - p_j} u(x_i) \text{ by the induction hypothesis} \\ &= \sum_{i=1}^k p_i u(x_i) \end{aligned}$$

□